Hoare/CPS_Hoare_Step.thy
@@ -71,4 +71,143 @@ next
   thus ?case by auto
 qed
 
+lemma Excp_1' : 
+  assumes H: "sem_exec_c_p gs m1 1 m2"
+  shows  "sem_step_p gs m1 m2"
+  using H
+proof(cases rule: sem_exec_c_p.cases)
+  case Excp_0
+  then show ?thesis by auto
+next
+  case (Excp_Suc m2' n)
+
+  have "sem_exec_c_p gs m2' 0 m2"
+    using Excp_Suc by auto
+
+  hence "m2' = m2" 
+    by(cases rule: sem_exec_c_p.cases; auto)
+
+  then show ?thesis using Excp_Suc by auto
+qed
+
+
+lemma exec_c_p_split :
+  assumes H : "sem_exec_c_p gs m1 n m3"
+  assumes Hj : "j \<le> n"
+  shows "\<exists> m2 . sem_exec_c_p gs m1 j m2 \<and> sem_exec_c_p gs m2 (n - j) m3"
+  using H Hj
+proof(induction arbitrary: j rule: sem_exec_c_p.induct)
+  case (Excp_0 m)
+
+  have "sem_exec_c_p gs m j m \<and> sem_exec_c_p gs m (0 - j) m"
+    using sem_exec_c_p.intros(1)[of gs m] Excp_0
+    by auto
+
+  then show ?case by blast
+next
+  case (Excp_Suc m1 m2 n m3)
+  then show ?case 
+  proof(cases j)
+    case 0
+
+    have C1 : "sem_exec_c_p gs m1 0 m1"
+      using sem_exec_c_p.intros(1)[of gs m1] by auto
+
+    have C2 : "sem_exec_c_p gs m1 (Suc n) m3" using sem_exec_c_p.intros(2)[OF Excp_Suc(1) Excp_Suc(2)]
+      by auto
+
+    have "sem_exec_c_p gs m1 j m1 \<and> sem_exec_c_p gs m1 (Suc n - j) m3"
+      using C1 C2 0 by auto
+
+    then show ?thesis by blast
+
+  next
+    case (Suc j')
+
+    hence Leq : "j' \<le> n" using Excp_Suc by auto
+
+    obtain m2x where M2x1 : "sem_exec_c_p gs m2 j' m2x" and M2x2 : "sem_exec_c_p gs m2x (n - j') m3"
+      using Excp_Suc.IH[OF Leq]
+      by auto
+
+    have "sem_exec_c_p gs m1 (j' + 1) m2x" using sem_exec_c_p.intros(2)[OF Excp_Suc(1) M2x1]
+      by auto
+
+    hence C1' : "sem_exec_c_p gs m1 (j) m2x" using Suc by auto
+
+    have C2' : "sem_exec_c_p gs m2x (Suc n - j) m3" using M2x2 Suc Excp_Suc.prems
+      by auto
+
+    show ?thesis using C1' C2' by blast
+
+  qed
+qed
+
+lemma exec_c_p_determ :
+  assumes H1 : "sem_exec_c_p gs m1 n m2"
+  assumes H2 : "sem_exec_c_p gs m1 n m2'"
+  shows "m2 = m2'" using H1 H2
+proof(induction arbitrary: m2' rule: sem_exec_c_p.induct)
+  case (Excp_0 m)
+  then show ?case 
+    by(cases rule: sem_exec_c_p.cases; auto)
+next
+  case (Excp_Suc m1 m2 n m3)
+
+  obtain m2_copy
+    where M2_copy1 : "sem_exec_c_p gs m1 1 m2_copy" and 
+      M2_copy2 :"sem_exec_c_p gs m2_copy (Suc n - 1) m2'"
+    using exec_c_p_split[OF Excp_Suc.prems, of 1]
+    by auto
+
+  have Step' : "sem_step_p gs m1 m2_copy" using M2_copy1
+  proof(cases rule: sem_exec_c_p.cases)
+    case Excp_0
+    then show ?thesis by auto
+  next
+    case Excp_Suc' : (Excp_Suc m2z nz)
+
+    then have "sem_exec_c_p gs m2z 0 m2_copy"
+      by auto
+
+    hence M2_eq : "m2z = m2_copy"
+      by(cases rule: sem_exec_c_p.cases; auto)
+
+    then show ?thesis using Excp_Suc' by auto  
+  qed
+
+  have M2_eq : "m2 = m2_copy"
+    using determE[OF sem_step_determ Step', of m2] Excp_Suc.hyps(1)
+    by auto
+
+  hence M2_copy2' : "sem_exec_c_p gs m2 (n) m2'"
+    using M2_copy2 by auto
+
+  show ?case using Excp_Suc.IH[OF M2_copy2'] by auto
+qed
+
+definition safe_for :: "('syn, 'mstate) semc \<Rightarrow> ('syn, 'mstate) control \<Rightarrow> nat \<Rightarrow> bool" where
+"safe_for gs m n =
+  (\<forall> n' m' . n' < n \<longrightarrow> sem_exec_c_p gs m n' m' \<longrightarrow> imm_safe gs m')"
+
+lemma safe_forI [intro]:
+  assumes H : "\<And> n' m' . n' < n \<Longrightarrow> sem_exec_c_p gs m n' m' \<Longrightarrow> imm_safe gs m'"
+  shows "safe_for gs m n" using H unfolding safe_for_def
+  by auto
+
+lemma safe_forD :
+  assumes H : "safe_for gs m n"
+  assumes Hlt : "n' < n"
+  assumes Hx : "sem_exec_c_p gs m n' m'"
+  shows "imm_safe gs m'" using H Hx Hlt
+  unfolding safe_for_def by blast
+
+lemma safe_for_safe : "(\<And> n . safe_for gs m n) \<Longrightarrow> safe gs m"
+  sorry
+
+lemma safe_safe_for : "safe gs m \<Longrightarrow> safe_for gs m n"
+  sorry
+
+
+
 end
